Update Submission.thy

homework/08/Submission.thy
@@ -5,17 +5,19 @@ begin
 inductive
   big_step :: "com \<times> state \<Rightarrow> state \<Rightarrow> bool" (infix "\<Rightarrow>" 55)
 where
-Skip:    "(SKIP,s) \<Rightarrow> s" |
-Assign:  "(x ::= a,s) \<Rightarrow> s(x := aval a s)" |
-Seq:    "\<lbrakk> (c\<^sub>1,s\<^sub>1) \<Rightarrow> s\<^sub>2; (c\<^sub>2,s\<^sub>2) \<Rightarrow> s\<^sub>3 \<rbrakk> \<Longrightarrow> (c\<^sub>1;;c\<^sub>2, s\<^sub>1) \<Rightarrow> s\<^sub>3" |
-IfTrue:  "\<lbrakk> bval b s;  (c\<^sub>1,s) \<Rightarrow> t \<rbrakk> \<Longrightarrow> (IF b THEN c\<^sub>1 ELSE c\<^sub>2, s) \<Rightarrow> t" |
-IfFalse: "\<lbrakk> \<not>bval b s;  (c\<^sub>2,s) \<Rightarrow> t \<rbrakk> \<Longrightarrow> (IF b THEN c\<^sub>1 ELSE c\<^sub>2, s) \<Rightarrow> t" |
-WhileFalse: "\<not>bval b s \<Longrightarrow> (WHILE b DO c,s) \<Rightarrow> s" |
-WhileTrue:  "\<lbrakk> bval b s\<^sub>1;  (c,s\<^sub>1) \<Rightarrow> s\<^sub>2;  (WHILE b DO c, s\<^sub>2) \<Rightarrow> s\<^sub>3 \<rbrakk> \<Longrightarrow> (WHILE b DO c, s\<^sub>1) \<Rightarrow> s\<^sub>3" |
-OrLeft: "\<lbrakk> (c\<^sub>1,s) \<Rightarrow> s' \<rbrakk> \<Longrightarrow> (c\<^sub>1 OR c\<^sub>2,s) \<Rightarrow> s'" |
-OrRight: "\<lbrakk> (c\<^sub>2,s) \<Rightarrow> s' \<rbrakk> \<Longrightarrow> (c\<^sub>1 OR c\<^sub>2,s) \<Rightarrow> s'" |
-Assume: "bval b s \<Longrightarrow> (ASSUME b, s) \<Rightarrow> s" |
-\<comment> \<open>Your cases here:\<close>
+Skip:         "(SKIP,s) \<Rightarrow> s" |
+Assign:       "(x ::= a,s) \<Rightarrow> s(x := aval a s)" |
+Seq:          "\<lbrakk> (c\<^sub>1,s\<^sub>1) \<Rightarrow> s\<^sub>2; (c\<^sub>2,s\<^sub>2) \<Rightarrow> s\<^sub>3 \<rbrakk> \<Longrightarrow> (c\<^sub>1;;c\<^sub>2, s\<^sub>1) \<Rightarrow> s\<^sub>3" |
+IfTrue:       "\<lbrakk> bval b s;  (c\<^sub>1,s) \<Rightarrow> t \<rbrakk> \<Longrightarrow> (IF b THEN c\<^sub>1 ELSE c\<^sub>2, s) \<Rightarrow> t" |
+IfFalse:      "\<lbrakk> \<not>bval b s;  (c\<^sub>2,s) \<Rightarrow> t \<rbrakk> \<Longrightarrow> (IF b THEN c\<^sub>1 ELSE c\<^sub>2, s) \<Rightarrow> t" |
+WhileFalse:   "\<not>bval b s \<Longrightarrow> (WHILE b DO c,s) \<Rightarrow> s" |
+WhileTrue:    "\<lbrakk> bval b s\<^sub>1;  (c,s\<^sub>1) \<Rightarrow> s\<^sub>2;  (WHILE b DO c, s\<^sub>2) \<Rightarrow> s\<^sub>3 \<rbrakk> \<Longrightarrow> (WHILE b DO c, s\<^sub>1) \<Rightarrow> s\<^sub>3" |
+OrLeft:       "\<lbrakk> (c\<^sub>1,s) \<Rightarrow> s' \<rbrakk> \<Longrightarrow> (c\<^sub>1 OR c\<^sub>2,s) \<Rightarrow> s'" |
+OrRight:      "\<lbrakk> (c\<^sub>2,s) \<Rightarrow> s' \<rbrakk> \<Longrightarrow> (c\<^sub>1 OR c\<^sub>2,s) \<Rightarrow> s'" |
+Assume:       "bval b s \<Longrightarrow> (ASSUME b, s) \<Rightarrow> s" |
+LoopBreak:    "(LOOP c,s) \<Rightarrow> s" |
+LoopContinue: "\<lbrakk> (c,s\<^sub>1) \<Rightarrow> s\<^sub>2;  (LOOP c, s\<^sub>2) \<Rightarrow> s\<^sub>3 \<rbrakk> \<Longrightarrow> (LOOP c, s\<^sub>1) \<Rightarrow> s\<^sub>3"
+
 declare big_step.intros [intro]
 lemmas big_step_induct = big_step.induct[split_format(complete)]
 
@@ -25,8 +27,15 @@ inductive_cases SeqE[elim!]: "(c1;;c2,s1) \<Rightarrow> s3"
 inductive_cases OrE: "(c1 OR c2,s1) \<Rightarrow> s3"
 inductive_cases IfE[elim!]: "(IF b THEN c1 ELSE c2,s) \<Rightarrow> t"
 inductive_cases WhileE[elim]: "(WHILE b DO c,s) \<Rightarrow> t"
+inductive_cases LoopE: "(LOOP c, s) \<Rightarrow> t"
 
 type_synonym com_den = "(state \<times> state) set"
+
+definition W :: "(state \<Rightarrow> bool) \<Rightarrow> com_den \<Rightarrow> (com_den \<Rightarrow> com_den)" where
+  "W db dc = (\<lambda>dw. {(s,t). if db s then (s,t) \<in> dc O dw else s=t})"
+
+definition L :: "com_den \<Rightarrow> (com_den \<Rightarrow> com_den)" where
+  "L dc = (\<lambda>dl. {(s,t). (s,t) \<in> dc O dl} \<union> {(s,t). s=t})"
 
 fun D :: "com \<Rightarrow> com_den" where
 "D SKIP   = Id" |
@@ -34,9 +43,63 @@ fun D :: "com \<Rightarrow> com_den" where
 "D (c1;;c2)  = D(c1) O D(c2)" |
 "D (IF b THEN c1 ELSE c2)
  = {(s,t). if bval b s then (s,t) \<in> D c1 else (s,t) \<in> D c2}" |
-"D (WHILE b DO c) = lfp (W (bval b) (D c))"
-\<comment> \<open>Your cases here:\<close>
-| "D _ = undefined"
+"D (WHILE b DO c) = lfp (W (bval b) (D c))" |
+"D (c1 OR c2) = (D c1) \<union> (D c2)" |
+"D (ASSUME b) = {(s,t). bval b s \<and> s = t}" |
+"D (LOOP c) = lfp (L (D c))"
+
+lemma W_mono: "mono (W b r)"
+by (unfold W_def mono_def) auto
+
+lemma D_While_If:
+  "D(WHILE b DO c) = D(IF b THEN c;;WHILE b DO c ELSE SKIP)"
+proof-
+  let ?w = "WHILE b DO c" let ?f = "W (bval b) (D c)"
+  have "D ?w = lfp ?f" by simp
+  also have "\<dots> = ?f (lfp ?f)" by(rule lfp_unfold [OF W_mono])
+  also have "\<dots> = D(IF b THEN c;;?w ELSE SKIP)" by (simp add: W_def)
+  finally show ?thesis .
+qed
+
+lemma D_if_big_step:  "(c,s) \<Rightarrow> t \<Longrightarrow> (s,t) \<in> D(c)"
+proof (induction rule: big_step_induct)
+  case WhileFalse
+  with D_While_If show ?case by auto
+next
+  case WhileTrue
+  show ?case unfolding D_While_If using WhileTrue by auto
+next
+  case (LoopBreak c s)
+  then show ?case sorry
+next
+  case (LoopContinue c s\<^sub>1 s\<^sub>2 s\<^sub>3)
+  then show ?case sorry
+qed auto
+
+abbreviation Big_step :: "com \<Rightarrow> com_den" where
+"Big_step c \<equiv> {(s,t). (c,s) \<Rightarrow> t}"
+
+lemma Big_step_if_D:  "(s,t) \<in> D(c) \<Longrightarrow> (s,t) \<in> Big_step c"
+proof (induction c arbitrary: s t)
+  case Seq thus ?case by fastforce
+next
+  case (While b c)
+  let ?B = "Big_step (WHILE b DO c)" let ?f = "W (bval b) (D c)"
+  have "?f ?B \<subseteq> ?B" using While.IH by (auto simp: W_def)
+  from lfp_lowerbound[where ?f = "?f", OF this] While.prems
+  show ?case by auto
+next
+  case (ASSUME b)
+  show ?case
+    using ASSUME by auto
+next
+  case (Loop c)
+  show ?case sorry
+qed (auto split: if_splits)
+
+theorem denotational_is_big_step:
+  "(s,t) \<in> D(c)  =  ((c,s) \<Rightarrow> t)"
+by (metis D_if_big_step Big_step_if_D[simplified])
 
 theorem denotational_is_big_step:
   "(s,t) \<in> D(c)  =  ((c,s) \<Rightarrow> t)"
